further tuned mk_db

src/verified.ml
@@ -111,9 +111,8 @@ module Monitor : sig
   val integer_of_int : int -> Z.t
   val interval : nat -> enat -> i
   val mk_db :
-    ('a -> (char list) list) ->
-      ('a -> char list -> (event_data list) set) ->
-        'a -> ((char list), ((event_data list) set list)) mapping
+    (char list * (event_data list) set) list ->
+      ((char list), ((event_data list) set list)) mapping
   val mstep :
     ((char list), ((event_data list) set list)) mapping * nat ->
       ((nat *
@@ -3458,7 +3457,7 @@ and rbt_comp_del_from_right
 
 let rec rbt_comp_delete c k t = paint B (rbt_comp_del c k t);;
 
-let rec deleteb _A
+let rec deletec _A
   xb xc =
     Mapping_RBTa (rbt_comp_delete (the (ccompare _A)) xb (impl_ofa _A xc));;
 
@@ -3501,7 +3500,7 @@ and remove (_A1, _A2)
           with None ->
             failwith "remove RBT_set: ccompare = None"
               (fun _ -> remove (_A1, _A2) x (RBT_set rbt))
-          | Some _ -> RBT_set (deleteb _A2 x rbt))
+          | Some _ -> RBT_set (deletec _A2 x rbt))
     | x, DList_set dxs ->
         (match ceq _A1
           with None ->
@@ -3907,6 +3906,8 @@ let rec rpd
         sup_seta (ceq_mregex, ccompare_mregex) (mTimesL r (rpd s)) (rpd r)
     | MStar r -> mTimesL (MStar r) (rpd r);;
 
+let rec delete _A k = filtera (fun (ka, _) -> not (eq _A k ka));;
+
 let rec update _A
   k v x2 = match k, v, x2 with k, v, [] -> [(k, v)]
     | k, v, p :: ps ->
@@ -4043,17 +4044,17 @@ let rec delete_aux _A
     | ka, (k, v) :: xs ->
         (if eq _A ka k then xs else (k, v) :: delete_aux _A ka xs);;
 
-let rec deletea _A xb xc = Alist (delete_aux _A xb (impl_of xc));;
+let rec deleteb _A xb xc = Alist (delete_aux _A xb (impl_of xc));;
 
-let rec delete (_A1, _A2)
+let rec deletea (_A1, _A2)
   k x1 = match k, x1 with
     k, RBT_Mapping t ->
       (match ccompare _A1
         with None ->
           failwith "delete RBT_Mapping: ccompare = None"
-            (fun _ -> delete (_A1, _A2) k (RBT_Mapping t))
-        | Some _ -> RBT_Mapping (deleteb _A1 k t))
-    | k, Assoc_List_Mapping al -> Assoc_List_Mapping (deletea _A2 k al)
+            (fun _ -> deletea (_A1, _A2) k (RBT_Mapping t))
+        | Some _ -> RBT_Mapping (deletec _A1 k t))
+    | k, Assoc_List_Mapping al -> Assoc_List_Mapping (deleteb _A2 k al)
     | k, Mapping m -> Mapping (fun_upd _A2 m k None);;
 
 let rec filterb _A
@@ -4161,6 +4162,9 @@ let rec restrict
   a v = mapa (fun i ->
                (if member (ceq_nat, ccompare_nat) i a then nth v i else None))
           (upt zero_nata (size_list v));;
+
+let rec clearjunk _A = function [] -> []
+                       | p :: ps -> p :: clearjunk _A (delete _A (fst p) ps);;
 
 let rec combine _B
   f (RBT_Mapping t) (RBT_Mapping u) =
@@ -5326,7 +5330,7 @@ let rec eval_step_mmuaux (_A1, _A2)
            a2_map
          in
        let a2_mapb =
-         delete (ccompare_nat, equal_nat) (minus_nata tp len) a2_mapa in
+         deletea (ccompare_nat, equal_nat) (minus_nata tp len) a2_mapa in
         (tp, (tl_queue tssa,
                (minus_nata len one_nata,
                  (maskL,
@@ -6552,7 +6556,7 @@ let rec filter_cfi _B (_A1, _A2)
   xa = Abs_comp_fun_idem
          (fun a m ->
            (match lookupa (_A1, _A2) m a with None -> m
-             | Some u -> (if eq _B xa u then delete (_A1, _A2) a m else m)));;
+             | Some u -> (if eq _B xa u then deletea (_A1, _A2) a m else m)));;
 
 let rec filter_set (_A1, _A2, _A3, _A4) _B
   m a t =
@@ -6593,7 +6597,7 @@ let rec add_new_ts_mmsaux (_A1, _A2, _A3)
     add_new_ts_mmsauxa (_A1, _A2, _A3) args nt
       (shift_end (_A1, _A2, _A3) args nt aux);;
 
-let rec filter_not_in_cfi (_A1, _A2) = Abs_comp_fun_idem (delete (_A1, _A2));;
+let rec filter_not_in_cfi (_A1, _A2) = Abs_comp_fun_idem (deletea (_A1, _A2));;
 
 let rec filter_join (_A1, _A2, _A3, _A4)
   pos a m =
@@ -7416,19 +7420,17 @@ let rec minit
   phi = (let n = nfv phi in Mstate_ext (zero_nata, minit0 n phi, n, ()));;
 
 let rec mk_db
-  get_names get_table t =
-    of_alist
-      ((ccompare_list ccompare_char), (equal_list equal_char),
-        mapping_impl_list)
-      (map_filter
-        (fun n ->
-          (let x = get_table t n in
+  t = of_alist
+        ((ccompare_list ccompare_char), (equal_list equal_char),
+          mapping_impl_list)
+        (map_filter
+          (fun (p, x) ->
             (if is_empty
                   (card_UNIV_list, (ceq_list ceq_event_data),
                     (cproper_interval_list ccompare_event_data))
                   x
-              then None else Some (n, [x]))))
-        (get_names t));;
+              then None else Some (p, [x])))
+          (clearjunk (equal_list equal_char) t));;
 
 let rec mstate_n (Mstate_ext (mstate_i, mstate_m, mstate_n, more)) = mstate_n;;
 
